Logic/Modal/Normal/ModalCube.lean
@@ -6,58 +6,203 @@
  * <https://plato.stanford.edu/entries/logic-modal/#MapRelBetModLog>
 -/
 
-import Logic.Modal.Normal.HilbertStyle
+import Logic.Modal.Normal.Soundness
+import Logic.Modal.Normal.Completeness
 
 namespace LO.Modal.Normal
 
-open Hilbert
+def LogicalStrong {β} (Λ₁ Λ₂ : AxiomSet β) := ∀ {α}, ∀ (p : Formula β), (⊧ᴹ[(𝔽(Λ₁) : FrameClass α)] p) → (⊧ᴹ[(𝔽(Λ₂) : FrameClass α)] p)
+infix:20 " ≤ᴸ " => LogicalStrong
 
-variable {F : Type u} [DecidableEq F] [ModalLogicSymbol F] [NegDefinition F] [ModalDuality F] (Bew : Set F → F → Type*)
+namespace LogicalStrong
 
-section LogicS5
+instance : IsPreorder (AxiomSet β) (· ≤ᴸ ·) where
+  refl := by simp_all [LogicalStrong];
+  trans := by intro Λ₁ Λ₂ Λ₃ h₁₂ h₂₃ _ p hF; exact h₂₃ p (h₁₂ p hF);
 
-instance [LogicS5.Hilbert Bew] : HasAxiomD Bew where
-  D _ _ := by sorry;
+variable {α β : Type u}
+variable {Λ₁ Λ₂ : AxiomSet β}
+variable [Inhabited α] [DecidableEq β]
 
-instance [LogicS5.Hilbert Bew] : HasAxiomB Bew where
-  B _ p := by sorry;
+lemma iff : (Λ₁ ≤ᴸ Λ₂) ↔ (∀ {α}, ∀ {F : Frame α}, (F ∈ 𝔽(Λ₂) → F ∈ (𝔽(Λ₁)))) := by
+  constructor;
+  . intro h _ F hF₂ p hp;
+    exact h p (by simp [Formula.FrameClasses]; aesop) F hF₂;
+  . intro h₁ _ p h₂ F hF₂;
+    have : F ∈ 𝔽(Λ₁) := h₁ hF₂;
+    exact h₂ F $ h₁ hF₂;
 
-instance [LogicS5.Hilbert Bew] : HasAxiom4 Bew where
-  A4 _ _ := by sorry;
+lemma not_iff : ¬(Λ₁ ≤ᴸ Λ₂) ↔ (∃ α, ∃ F ∈ 𝔽(Λ₂), (F : Frame α) ∉ 𝔽(Λ₁)) := by simpa using iff.not
 
-/-- `𝐒𝟓` Without `𝐓` -/
-class LogicKDB5.Hilbert extends LogicK.Hilbert Bew, HasAxiomD Bew, HasAxiomB Bew, HasAxiom5 Bew
+variable (hS : Λ₁ ≤ᴸ Λ₂) {Γ : Theory β} {p : Formula β}
 
-instance [LogicKDB5.Hilbert Bew] : HasAxiom4 Bew where
-  A4 _ _ := by sorry;
+lemma consequence : (Γ ⊨ᴹ[(𝔽(Λ₁) : FrameClass α)] p) → (Γ ⊨ᴹ[(𝔽(Λ₂) : FrameClass α)] p) := by
+  intro h F hF₁;
+  exact h F $ iff.mp hS hF₁;
 
-instance [LogicKDB5.Hilbert Bew] : LogicS5.Hilbert Bew where
-  K _ p q := by sorry;
-  T _ p := by sorry;
-  A5 _ p := by sorry;
+lemma deducible (hComp : Completeness Λ₂ (𝔽(Λ₂) : FrameClass α)) (hd : Γ ⊢ᴹ[Λ₁]! p) : Γ ⊢ᴹ[Λ₂]! p := by
+  apply hComp;
+  exact consequence hS $ AxiomSet.sounds hd;
 
-instance [LogicS5.Hilbert Bew] : LogicKDB5.Hilbert Bew where
+end LogicalStrong
 
-/-- `𝐒𝟓` Without `𝟓` -/
-class LogicKT4B.Hilbert extends LogicK.Hilbert Bew, HasAxiomT Bew, HasAxiom4 Bew, HasAxiomB Bew
+abbrev LogicalStrictStrong (Λ₁ Λ₂ : AxiomSet β) := (Λ₁ ≤ᴸ Λ₂) ∧ ¬(Λ₂ ≤ᴸ Λ₁)
+infix:20 " <ᴸ " => LogicalStrictStrong
 
-instance [LogicKT4B.Hilbert Bew] : LogicS5.Hilbert Bew where
-  K _ _ := by sorry;
-  T _ _ := by sorry;
-  A5 _ _ := by sorry;
+namespace LogicStrictStronger
 
-instance [LogicS5.Hilbert Bew] : LogicKT4B.Hilbert Bew where
+instance : IsStrictOrder (AxiomSet β) (· <ᴸ ·) where
+  irrefl := by simp [LogicalStrong]
+  trans := by
+    simp [LogicalStrong];
+    intro Λ₁ Λ₂ Λ₃ h₁₂ _ _ _ _ h₂₃ α₂ y _ _;
+    constructor;
+    . intro _ p h₁;
+      exact h₂₃ p $ h₁₂ p h₁;
+    . simp [LogicalStrong];
+      existsi α₂, y;
+      constructor;
+      . simpa;
+      . by_contra hn₁;
+        have := h₁₂ y hn₁;
+        contradiction;
 
--- Without `𝐓` and `𝟓`
-class LogicKD4B.Hilbert extends LogicK.Hilbert Bew, HasAxiomD Bew, HasAxiom4 Bew, HasAxiomB Bew
+variable {Λ₁ Λ₂ : AxiomSet β} (hS : Λ₁ <ᴸ Λ₂)
+variable [DecidableEq β]
 
-instance [LogicKD4B.Hilbert Bew] : LogicS5.Hilbert Bew where
-  K _ _ := by sorry;
-  T _ _ := by sorry;
-  A5 _ _ := by sorry;
+end LogicStrictStronger
 
-instance [LogicS5.Hilbert Bew] : LogicKD4B.Hilbert Bew where
+abbrev LogicalEquivalence (Λ₁ Λ₂ : AxiomSet β) := (Λ₁ ≤ᴸ Λ₂) ∧ (Λ₂ ≤ᴸ Λ₁)
+infix:75 " =ᴸ " => LogicalEquivalence
 
-end LogicS5
+namespace LogicalEquivalence
+
+instance : IsEquiv (AxiomSet β) (· =ᴸ ·) where
+  refl := by simp; apply IsRefl.refl;
+  trans := by
+    simp; intros;
+    constructor <;> simp_all [LogicalStrong];
+  symm := by
+    simp; intros;
+    constructor <;> simp_all;
+
+variable {α₁ α₂ β} [Inhabited α₁] [Inhabited α₂] [DecidableEq β]
+
+lemma deducible
+  {Λ₁ Λ₂ : AxiomSet β} (h : Λ₁ =ᴸ Λ₂)
+  (hComp₁ : Completeness Λ₁ (𝔽(Λ₁) : FrameClass α₁))
+  (hComp₂ : Completeness Λ₂ (𝔽(Λ₂) : FrameClass α₂))
+  {Γ} {p : Formula β} : (Γ ⊢ᴹ[Λ₁]! p) ↔ (Γ ⊢ᴹ[Λ₂]! p) := by
+  constructor;
+  . apply LogicalStrong.deducible h.1 hComp₂
+  . apply LogicalStrong.deducible h.2 hComp₁
+
+end LogicalEquivalence
+
+variable {α β : Type u} [Inhabited β] [DecidableEq β]
+variable {p : Formula β}
+
+def LogicKT : AxiomSet α := 𝐊 ∪ 𝐓
+notation "𝐊𝐓" => LogicKT
+
+namespace LogicKT
+
+@[simp] lemma subset_K : 𝐊 ⊆ (𝐊𝐓 : AxiomSet α) := by simp [LogicKT]
+@[simp] lemma subset_T : 𝐓 ⊆ (𝐊𝐓 : AxiomSet α) := by simp [LogicKT]
+
+instance FrameClassDefinability : @FrameClassDefinability α β 𝐊𝐓 (λ F => (Reflexive F)) := by
+  intro F;
+  simp [LogicKT, AxiomSetFrameClass.union];
+  have := AxiomK.defines β F;
+  have := AxiomT.defines β F;
+  aesop;
+
+end LogicKT
+
+theorem sstrong_KD_KT : (𝐊𝐃 : AxiomSet (Fin 2)) <ᴸ 𝐊𝐓 := by
+  constructor;
+  . apply LogicalStrong.iff.mpr;
+    intro _ F hF;
+    obtain hRefl := LogicKT.FrameClassDefinability.mpr hF;
+    apply LogicKD.FrameClassDefinability.mp;
+    exact serial_of_refl hRefl;
+  . apply LogicalStrong.not_iff.mpr;
+    existsi _, (λ _ w₂ => w₂ = 1);
+    constructor;
+    . apply LogicKD.FrameClassDefinability.mp;
+      simp [Serial];
+    . apply LogicKT.FrameClassDefinability.not.mp;
+      simp [Reflexive]
+      existsi 0;
+      trivial;
+
+theorem sstrong_S4_S5 : (𝐒𝟒 : AxiomSet (Fin 3)) <ᴸ 𝐒𝟓 := by
+  constructor;
+  . apply LogicalStrong.iff.mpr;
+    intro _ F hF;
+    obtain ⟨hRefl, hEucl⟩ := LogicS5.FrameClassDefinability.mpr hF;
+    apply LogicS4.FrameClassDefinability.mp;
+    constructor;
+    . exact hRefl;
+    . exact trans_of_refl_eucl hRefl hEucl;
+  . apply LogicalStrong.not_iff.mpr;
+    existsi (Fin 3), (λ w₁ w₂ => (w₁ = w₂) ∨ (w₁ = 0 ∧ w₂ = 1) ∨ (w₁ = 0 ∧ w₂ = 2));
+    constructor;
+    . apply LogicS4.FrameClassDefinability.mp;
+      simp [Reflexive, Transitive];
+      trivial;
+    . apply LogicS5.FrameClassDefinability.not.mp;
+      simp [Reflexive, Euclidean];
+      existsi 0, 1, 2;
+      trivial;
+
+def LogicKT4B : AxiomSet α := 𝐊 ∪ 𝐓 ∪ 𝟒 ∪ 𝐁
+notation "𝐊𝐓𝟒𝐁" => LogicKT4B
+
+namespace LogicKT4B
+
+@[simp] lemma subset_K : 𝐊 ⊆ (𝐊𝐓𝟒𝐁 : AxiomSet α) := by simp [LogicKT4B, LogicK]
+@[simp] lemma subset_T : 𝐓 ⊆ (𝐊𝐓𝟒𝐁 : AxiomSet α) := by simp [LogicKT4B, LogicK]
+@[simp] lemma subset_4 : 𝟒 ⊆ (𝐊𝐓𝟒𝐁 : AxiomSet α) := by simp [LogicKT4B, LogicK]
+@[simp] lemma subset_B : 𝐁 ⊆ (𝐊𝐓𝟒𝐁 : AxiomSet α) := by simp [LogicKT4B, LogicK]
+
+instance FrameClassDefinability : @FrameClassDefinability α β 𝐊𝐓𝟒𝐁 (λ F => (Reflexive F ∧ Transitive F ∧ Symmetric F)) := by
+  intro F;
+  simp [LogicKT4B, AxiomSetFrameClass.tetraunion];
+  have := AxiomK.defines β F;
+  have := AxiomT.defines β F;
+  have := Axiom4.defines β F;
+  have := AxiomB.defines β F;
+  aesop;
+
+abbrev CanonicalModel {β} := Normal.CanonicalModel (𝐊𝐓𝟒𝐁 : AxiomSet β)
+theorem Hilbert.completes : @Completeness (MaximalConsistentTheory (𝐊𝐓𝟒𝐁 : AxiomSet β)) β 𝐊𝐓𝟒𝐁 (𝔽((𝐊𝐓𝟒𝐁 : AxiomSet β)) : FrameClass (MaximalConsistentTheory (𝐊𝐓𝟒𝐁 : AxiomSet β))) := by
+  apply completeness_def.mpr;
+  intro Γ hConsisΓ;
+  let ⟨Ω, hΩ⟩ := exists_maximal_consistent_theory hConsisΓ;
+  existsi CanonicalModel.frame;
+  constructor;
+  . apply FrameClassDefinability.mp; simp_all;
+  . existsi CanonicalModel.val, Ω;
+    apply truthlemma' (by simp) |>.mpr;
+    assumption;
+
+end LogicKT4B
+
+theorem equivalent_S5_KT4B : (𝐒𝟓 : AxiomSet β) =ᴸ 𝐊𝐓𝟒𝐁 := by
+  constructor;
+  . apply LogicalStrong.iff.mpr;
+    intro _ F hF;
+    obtain ⟨hRefl, hTrans, hSymm⟩ := LogicKT4B.FrameClassDefinability.mpr hF;
+    apply LogicS5.FrameClassDefinability.mp;
+    exact ⟨hRefl, eucl_of_symm_trans hSymm hTrans⟩
+  . apply LogicalStrong.iff.mpr;
+    intro _ F hF;
+    obtain ⟨hRefl, hEucl⟩ := LogicS5.FrameClassDefinability.mpr hF;
+    apply LogicKT4B.FrameClassDefinability.mp;
+    exact ⟨hRefl, trans_of_refl_eucl hRefl hEucl, symm_of_refl_eucl hRefl hEucl⟩
+
+theorem deducible_equivalent_S5_KT4B {Γ} {p : Formula β} : (Γ ⊢ᴹ[𝐒𝟓]! p) ↔ (Γ ⊢ᴹ[𝐊𝐓𝟒𝐁]! p) := by
+  exact LogicalEquivalence.deducible equivalent_S5_KT4B LogicS5.Hilbert.completes LogicKT4B.Hilbert.completes
 
 end LO.Modal.Normal
