Logic/Modal/Normal/Soundness.lean
@@ -7,41 +7,46 @@ namespace LO.Modal.Normal
 
 open Formula
 
-variable {α β} [Inhabited α] [DecidableEq α] [Inhabited β]
+variable {α β} [Inhabited α] [DecidableEq α]
 
-@[simp] def AxiomSet.Consistent (Λ : AxiomSet α) := ⊬ᴹ[Λ]! ⊥
+@[simp] def AxiomSet.Consistent (Λ : AxiomSet α) := ∅ ⊬ᴹ[Λ]! ⊥
 
 open AxiomSet
 
 variable {Λ : AxiomSet α} {p : Formula α}
 
-open FrameClasses in
-private lemma AxiomSet.soundsAux {Γ : Theory α} (hΓ : Γ = ∅) (d : Γ ⊢ᴹ[Λ]! p) : (⊧ᴹ[(𝔽(Λ) : FrameClass β)] p) := by
+theorem AxiomSet.sounds (d : Γ ⊢ᴹ[Λ]! p) : (Γ ⊨ᴹ[(𝔽(Λ) : FrameClass β)] p) := by
   induction d.some with
-  | axm => subst hΓ; contradiction;
-  | maxm => intros _ hF _ _; apply hF; simpa;
-  | modus_ponens h₁ h₂ ih₁ ih₂ => exact modus_ponens (ih₁ (by simp_all) ⟨h₁⟩) (ih₂ (by simp_all) ⟨h₂⟩);
-  | necessitation h ih => exact necessitation (ih rfl ⟨h⟩);
-  | verum => exact verum;
-  | imply₁ => exact imply₁;
-  | imply₂ => exact imply₂;
-  | conj₁ => exact conj₁;
-  | conj₂ => exact conj₂;
-  | conj₃ => exact conj₃;
-  | disj₁ => exact disj₁;
-  | disj₂ => exact disj₂;
-  | disj₃ => exact disj₃;
-  | dne => exact dne;
-
-theorem AxiomSet.sounds (d : ⊢ᴹ[Λ]! p) : (⊧ᴹ[(𝔽(Λ) : FrameClass β)] p) := AxiomSet.soundsAux rfl d
+  | axm h => intro _ _ _ _ hΓ; exact hΓ _ h;
+  | maxm h => intro _ hF _ _ _; apply hF; simpa;
+  | @modus_ponens Γ₁ Γ₂ p q h₁ h₂ ih₁ ih₂ =>
+    have hpq := FrameClassConsequence.weakening (show Γ₁ ⊆ (Γ₁ ∪ Γ₂) by simp) $ ih₁ ⟨h₁⟩;
+    have hp := FrameClassConsequence.weakening (show Γ₂ ⊆ (Γ₁ ∪ Γ₂) by simp) $ ih₂ ⟨h₂⟩;
+    exact FrameClassConsequence.modus_ponens' hpq hp;
+  | necessitation h ih =>
+    have := ih ⟨h⟩;
+    exact FrameClassConsequence.necessitation _ this
+  | _ =>
+    simp only [FrameClassConsequence, FrameConsequence];
+    intros;
+    try first
+    | apply Models.verum;
+    | apply Models.imply₁;
+    | apply Models.imply₂;
+    | apply Models.conj₁;
+    | apply Models.conj₂;
+    | apply Models.conj₃;
+    | apply Models.disj₁;
+    | apply Models.disj₂;
+    | apply Models.disj₃;
+    | apply Models.dne;
 
 lemma AxiomSet.consistent (β) [Inhabited β] [h : Nonempty (𝔽(Λ) : FrameClass β)] : Consistent Λ := by
-  by_contra hC;
-  suffices h : ∃ (F : Frame β), ⊧ᴹ[F] (⊥ : Formula α) by simp_all;
-  obtain ⟨F, hF⟩ := h.some;
-  existsi F;
-  apply AxiomSet.sounds (by simpa using hC);
-  simpa;
+  intro h;
+  have : ∅ ⊨ᴹ[(𝔽(Λ) : FrameClass β)] ⊥ := AxiomSet.sounds h;
+  simp_all [FrameClassConsequence, FrameConsequence]
+
+variable [Inhabited β]
 
 theorem LogicK.consistent : Consistent (𝐊 : AxiomSet α) := AxiomSet.consistent β
 theorem LogicKD.consistent : Consistent (𝐊𝐃 : AxiomSet α) := AxiomSet.consistent β
